Session 16 delivered

Session16Exercises/williams-0.dfy
@@ -16,23 +16,22 @@ class Williams_heap {
     requires 0 <= j <= v.Length
     reads this, v
     {
-        //(next == 0 ==> model == multiset([])) &&
         this in repr && v in repr &&
         0 <= next <= v.Length && 
-        forall i | 2*j+1 <= i < next :: v[(i-1)/2] <= v[i] //&&
-        //forall i | j <=i <next :: v[i] in model
+        (forall i | 2*j+1 <= i < next :: v[(i-1)/2] <= v[i]) &&
+        model == multiset(v[..next])
     }
     
 
     constructor (size: nat) 
     ensures isHeap(0) && v.Length == size && next == 0
     ensures fresh (repr)
-    //ensures model == multiset([])
+    ensures model == multiset{}
     {
         v := new int [size];
         next := 0;
         repr := {this, v};
-        model := multiset([]);
+        model := multiset{};
     }
 
     function method min(): int
@@ -40,8 +39,36 @@ class Williams_heap {
     //reads repr
     requires isHeap(0)
     requires next > 0
+    //ensures min() in model
+    ensures forall i | 0<=i<next :: v[i] >= min() 
     {
+        assert forall i | 0<=i <next :: isHeap(i);
+        firstIsMin();
+        
+        //assert forall i | 0<i<next :: v[i] >= v[0];
         v[0]
+    }
+
+    lemma firstIsMin()
+    requires isHeap(0)
+    requires next > 0
+    ensures forall i | 0<i< next :: v[i] >= v[0]
+    {
+        forall i | 0<i< next ensures v[i] >= v[0]{
+            firstIsLessEqual(i);
+        }
+    }
+
+    lemma firstIsLessEqual(j:nat)
+    requires isHeap(0)
+    requires 0 < j < next
+    ensures v[j] >= v[0]
+    //ensures forall i | 0<=i< next :: v[i] >= v[0]
+    {
+        if (0 == (j-1)/2){}
+        else{
+            firstIsLessEqual((j-1)/2);
+        }
     }
 
     method insert (val: int)
@@ -54,21 +81,28 @@ class Williams_heap {
     ensures repr == old(repr) 
     //ensures v == old(v)
     ensures v.Length == old(v.Length)
+    ensures model == old(model) + multiset{val}
+    //ensures forall i | 0<=i<next :: v[i] >= min() 
     {
         v[next] := val; next := next + 1;
+        model := model + multiset{val};
+        assert model==multiset(v[..next]);
         float ();
     }
 
     method float()
     requires 0 < next <= v.Length
     requires this in repr && v in repr; // isHeap(0) does not hold here
+    requires model==multiset(v[..next])
     requires forall i | 0 < i < next-1 :: v[(i-1)/2] <= v[i]
     modifies v //this, v (modifying this dafny doesnt know if im creating a new object for v)
     //ensures repr == old(repr)
     ensures isHeap(0)
+    ensures model == old(model) == multiset(v[..next])
     {
         var j := next-1;
         while j > 0 && v[(j-1)/2] > v[j] 
+            invariant model == old(model) == multiset(v[..next])
             invariant 0 <= j <= next-1 < v.Length
             invariant forall i | 0 < i < next :: i != j ==> v[(i-1)/2] <= v[i]
             invariant j > 0 && 2*j+1< next ==> v[(j-1)/2] <= v[2*j+1] 
@@ -77,7 +111,7 @@ class Williams_heap {
             v[(j-1)/2], v[j] := v[j], v[(j-1)/2];
             j := (j-1)/2;
         }
-}
+    }
 
     method deleteMin ()
     requires isHeap(0)
@@ -87,8 +121,16 @@ class Williams_heap {
     ensures isHeap(0) 
     ensures next == old(next) - 1
     ensures repr == old(repr)
+    ensures model == old(model) - multiset{old(v[0])}
     {
-        v[0] := v[next-1]; next := next - 1;
+        ghost var pre := v[0];
+        assert pre in model;
+
+        
+        v[0] := v[next-1]; 
+        next := next - 1;
+        model := model - multiset{pre};
+        assert model == multiset(v[..next]);
         sink (0, next);
     }
 
@@ -96,13 +138,21 @@ class Williams_heap {
     method sink(s:nat, l:nat)
     requires 0 <= s <= l == next <= v.Length
     requires this in repr && v in repr    // isHeap(0) does not hold here
+    //requires next == 0 <==> model == multiset{}
+    //requires forall i | 0 <= i < next :: v[i] in model
+    requires model == multiset(v[..next])
     requires forall i | 0 < i < next :: (i-1)/2 != s ==> v[(i-1)/2] <= v[i]
     modifies v
     ensures repr == old(repr)
     ensures isHeap(s)
+    ensures model == old(model) == multiset(v[..next])
     {
+        //assert next == 0 ==> model == multiset([]);
         var j := s;
         while 2*j+1 < l 
+            //invariant forall i | 0 <= i < next :: v[i] in model
+            invariant model == old(model) == multiset(v[..next])
+            //invariant model == old(model)
             invariant forall k | 2*s+1 <= k < l :: (k-1)/2 != j ==> v[(k-1)/2] <= v[k]
             invariant j >= 2*s+1 && 2*j+1< l ==> v[(j-1)/2] <= v[2*j+1] 
             invariant j >= 2*s+1 && 2*j+2< l ==> v[(j-1)/2] <= v[2*j+2]
@@ -123,9 +173,17 @@ class Williams_heap {
     }
 }
 
+predicate sorted_seg(a:array<int>, i:int, j:int) //j not included
+requires 0 <= i <= j <= a.Length
+reads a
+{
+    forall l, k :: i <= l <= k < j ==> a[l] <= a[k]
+}
+
+
 method heapsort_with_extra_space (a: array<int>)
 modifies a
-//ensures sorted
+ensures sorted_seg(a, 0, a.Length)
 {
     var queue := new Williams_heap(a.Length);
     var i := 0;
@@ -140,13 +198,21 @@ modifies a
     }
     i := 0;
     while i < a.Length 
+        invariant 0<=i<=a.Length
+        invariant sorted_seg(a, 0, i)
+        invariant forall j, k | 0<=j<i && k in queue.model :: a[j] <= k
         invariant queue.isHeap(0) 
         invariant queue.next == a.Length - i
         invariant fresh(queue.repr)
     {
         assert queue.isHeap(0); 
         assert queue.next > 0;
+        queue.firstIsMin();
+        assert forall j | 0<j<queue.next ::queue.min()<=queue.v[j];
+        assert forall j, k | 0<=j<i && k in queue.model :: a[j] <= k;
         a[i] := queue.min(); 
+        assert a[i] in queue.model;
+        assert forall j | 0<=j<i :: a[j] <= a[i];
         queue.deleteMin();
         i := i + 1;
     }
