Session17Exercises/ExerciseReplace.dfy
@@ -1,0 +1,49 @@
+//Author: Clara Segura
+include "List.dfy"
+
+
+method replace(l:List,x:int,y:int)
+modifies l,l.Repr()
+requires l.Valid()
+requires forall x | x in l.Repr() :: allocated(x)
+
+ensures l.Valid() //inv
+
+//ensures: write the properties concerning the model
+//replace each occurrence of x by y, and leave the rest unchanged 
+ensures |l.Model()| == |old(l).Model()|
+ensures forall i| 0<=i<|old(l).Model()| && old(l).Model()[i]==x :: l.Model()[i]==y
+ensures forall i| 0<=i<|old(l).Model()| && old(l).Model()[i]!=x :: l.Model()[i]==old(l).Model()[i]
+
+ensures l.Iterators() >= old(l.Iterators())
+
+//copy this to invariant
+ensures forall x {:trigger x in l.Repr(), x in old(l.Repr())} | x in l.Repr() && x !in old(l.Repr()) :: fresh(x)
+ensures fresh(l.Repr()-old(l.Repr()))
+ensures forall x | x in l.Repr() :: allocated(x)
+{
+    var it:=l.Begin();
+    while(it.HasNext())
+    invariant l.Valid()
+    invariant it.Valid()
+    invariant it.Parent() == l
+    invariant l.Size() == old(l.Size())
+    decreases l.Size() - it.Index()
+    invariant it.Index() <= l.Size()
+    invariant l.Iterators() >= old(l.Iterators())
+    invariant forall x {:trigger x in l.Repr(), x in old(l.Repr())} | x in l.Repr() && x !in old(l.Repr()) :: fresh(x)
+    invariant fresh(l.Repr()-old(l.Repr()))
+    invariant forall x | x in l.Repr() :: allocated(x)
+    invariant forall i| 0<=i<it.Index() && old(l).Model()[i]==x :: l.Model()[i]==y
+    invariant forall i| 0<=i<it.Index() && old(l).Model()[i]!=x :: l.Model()[i]==old(l).Model()[i]
+    {
+        if(it.Peek() == x){
+            it.Set(y);
+        }
+        var xx:=it.Next();
+    }
+    
+}
+
+
+
